Launchbury/CorrectnessResourced.thy
@@ -6,31 +6,53 @@ begin
 theorem correctness:
   assumes "\<Gamma> : e \<Down>\<^bsub>L\<^esub> \<Delta> : z"
   and     "distinctVars \<Gamma>"
-  and     "fdom \<rho> - heapVars \<Gamma> \<subseteq> set L"
-  shows   "\<N>\<lbrakk>e\<rbrakk>\<^bsub>\<N>\<lbrace>\<Gamma>\<rbrace>\<rho>\<^esub> \<sqsubseteq> \<N>\<lbrakk>z\<rbrakk>\<^bsub>\<N>\<lbrace>\<Delta>\<rbrace>\<rho>\<^esub>" and "\<N>\<lbrace>\<Gamma>\<rbrace>\<rho> \<sqsubseteq> \<N>\<lbrace>\<Delta>\<rbrace>\<rho>"
+  and     "fv (\<Gamma>, e) - heapVars \<Gamma> \<subseteq> set L"
+  shows   "\<N>\<lbrakk>e\<rbrakk>\<^bsub>\<N>\<lbrace>\<Gamma>\<rbrace>\<rho>\<^esub> \<sqsubseteq> \<N>\<lbrakk>z\<rbrakk>\<^bsub>\<N>\<lbrace>\<Delta>\<rbrace>\<rho>\<^esub>" and "(\<N>\<lbrace>\<Gamma>\<rbrace>\<rho>) f|` (heapVars \<Gamma>) \<sqsubseteq> (\<N>\<lbrace>\<Delta>\<rbrace>\<rho>) f|` (heapVars \<Gamma>)"
   using assms
 proof(nominal_induct arbitrary: \<rho> rule:reds_distinct_strong_ind)
-case (Lambda \<Gamma> x e L)
+case Lambda
   case 1 show ?case..
   case 2 show ?case..
 next
 case (Application y \<Gamma> e x L \<Delta> \<Theta> z e')
   hence "y \<noteq> x" by (simp_all add: fresh_at_base)
 
+  have Gamma_subset: "heapVars \<Gamma> \<subseteq> heapVars \<Delta>"
+    by (rule reds_doesnt_forget[OF distinct_redsD1[OF Application.hyps(8)]])
+
   case 1
-  hence hyp1: "fdom \<rho> - heapVars \<Gamma> \<subseteq> set (x # L)" by auto
-  have hyp2: "fdom \<rho> - heapVars \<Delta> \<subseteq> set L"
-    using 1 reds_doesnt_forget[OF distinct_redsD1[OF Application.hyps(8)]]
-    by auto
+  hence prem1: "fv (\<Gamma>, e) - heapVars \<Gamma> \<subseteq> set (x#L)" by auto
+
+  from 1 Gamma_subset have *: "x \<in> set L \<or> x \<in> heapVars \<Delta>" by auto
+
+  have "fv (\<Delta>, e'[y::=x]) - heapVars \<Delta> \<subseteq> (fv (\<Delta>, Lam [y]. e') - heapVars \<Delta>) \<union> {x}"
+    by (auto dest!: set_mp[OF fv_subst_subset])
+  also have "\<dots> \<subseteq> (fv (\<Gamma>, e) - heapVars \<Gamma>) \<union> {x}"
+    using new_free_vars_on_heap[OF distinct_redsD1[OF Application.hyps(8)]] by auto
+  also have "\<dots> \<subseteq> set L \<union> {x}" using prem1 by auto
+  finally have "fv (\<Delta>, e'[y::=x]) - heapVars \<Delta> \<subseteq> set L \<union> {x}". 
+  with *
+  have prem2: "fv (\<Delta>, e'[y::=x]) - heapVars \<Delta> \<subseteq> set L" by auto
+  
+  have *: "(\<N>\<lbrace>\<Gamma>\<rbrace>\<rho> f! x) \<sqsubseteq> (\<N>\<lbrace>\<Delta>\<rbrace>\<rho> f! x)"
+  proof(cases "x \<in> heapVars \<Gamma>")
+    case True
+    thus ?thesis
+      using fmap_belowE[OF Application.hyps(10)[OF prem1], where \<rho>1 = \<rho> and x = x]
+      by simp
+  next
+    case False 
+    from False reds_avoids_live[OF distinct_redsD1[OF Application.hyps(8)] _ False] 
+    show ?thesis by (simp add: the_lookup_HSem_other)
+  qed
 
   have "\<N>\<lbrakk> App e x \<rbrakk>\<^bsub>\<N>\<lbrace>\<Gamma>\<rbrace>\<rho>\<^esub> = (\<Lambda> (C\<cdot>r). ((\<N>\<lbrakk> e \<rbrakk>\<^bsub>\<N>\<lbrace>\<Gamma>\<rbrace>\<rho>\<^esub>) \<cdot> r \<down>CFn C_restr\<cdot>r\<cdot>(\<N>\<lbrace>\<Gamma>\<rbrace>\<rho> f! x)) \<cdot> r)"
     by simp
   also have "\<dots> \<sqsubseteq> (\<Lambda> (C\<cdot>r). ((\<N>\<lbrakk> Lam [y]. e' \<rbrakk>\<^bsub>\<N>\<lbrace>\<Delta>\<rbrace>\<rho>\<^esub>) \<cdot> r \<down>CFn C_restr\<cdot>r\<cdot>(\<N>\<lbrace>\<Gamma>\<rbrace>\<rho> f! x)) \<cdot> r)"
-    using Application.hyps(9)[OF hyp1]
+    using Application.hyps(9)[OF prem1]
     by (fastforce intro: monofun_cfun_arg monofun_cfun_fun monofun_LAM)
   also have "\<dots> \<sqsubseteq> (\<Lambda> (C\<cdot>r). ((\<N>\<lbrakk> Lam [y]. e' \<rbrakk>\<^bsub>\<N>\<lbrace>\<Delta>\<rbrace>\<rho>\<^esub>) \<cdot> r \<down>CFn C_restr\<cdot>r\<cdot>(\<N>\<lbrace>\<Delta>\<rbrace>\<rho> f! x)) \<cdot> r)"
-    using fmap_belowE[OF Application.hyps(10)[OF hyp1]]
-    by (fastforce intro: monofun_cfun_arg monofun_cfun_fun monofun_LAM)
+    by (intro monofun_cfun_arg monofun_cfun_fun monofun_LAM *) simp_all
   also have "\<dots> = (\<Lambda> (C\<cdot>r). (((\<Lambda> (C \<cdot> r). CFn \<cdot> (\<Lambda> v. C_restr\<cdot>r\<cdot>(\<N>\<lbrakk> e' \<rbrakk>\<^bsub>(\<N>\<lbrace>\<Delta>\<rbrace>\<rho>)(y f\<mapsto> C_restr\<cdot>r\<cdot>v)\<^esub>)))) \<cdot> r \<down>CFn C_restr\<cdot>r\<cdot>(\<N>\<lbrace>\<Delta>\<rbrace>\<rho> f! x)) \<cdot> r)"
     by simp
   also have "\<dots> \<sqsubseteq> (\<Lambda> (C\<cdot>r). ((CFn \<cdot> (\<Lambda> v. C_restr\<cdot>r\<cdot>(\<N>\<lbrakk> e' \<rbrakk>\<^bsub>(\<N>\<lbrace>\<Delta>\<rbrace>\<rho>)(y f\<mapsto> C_restr\<cdot>r\<cdot>v)\<^esub>))) \<down>CFn C_restr\<cdot>r\<cdot>(\<N>\<lbrace>\<Delta>\<rbrace>\<rho> f! x)) \<cdot> r)"
@@ -56,12 +78,13 @@ case (Application y \<Gamma> e x L \<Delta> \<Theta> z e')
   also have "\<dots> \<sqsubseteq> \<N>\<lbrakk> e'[y ::= x] \<rbrakk>\<^bsub>(\<N>\<lbrace>\<Delta>\<rbrace>\<rho>)\<^esub>"
     by (subst eta_cfun, rule C_case_below)
   also have "\<dots> \<sqsubseteq> \<N>\<lbrakk> z \<rbrakk>\<^bsub>\<N>\<lbrace>\<Theta>\<rbrace>\<rho>\<^esub>"
-    by (rule Application.hyps(12)[OF hyp2])
+    by (rule Application.hyps(12)[OF prem2])
   finally
   show ?case.
   
-  show "\<N>\<lbrace>\<Gamma>\<rbrace>\<rho> \<sqsubseteq> \<N>\<lbrace>\<Theta>\<rbrace>\<rho>"
-    using Application.hyps(10)[OF hyp1] Application.hyps(13)[OF hyp2]
+  show "(\<N>\<lbrace>\<Gamma>\<rbrace>\<rho>) f|` (heapVars \<Gamma>) \<sqsubseteq> (\<N>\<lbrace>\<Theta>\<rbrace>\<rho>)  f|` (heapVars \<Gamma>)"
+    using Application.hyps(10)[OF prem1]
+          fmap_restr_below_subset[OF Gamma_subset Application.hyps(13)[OF prem2]]
     by (rule below_trans)
 next
 case (Variable x e \<Gamma> L \<Delta> z)
@@ -76,86 +99,49 @@ case (Variable x e \<Gamma> L \<Delta> z)
   have subset: "heapVars (delete x \<Gamma>) \<subseteq> heapVars \<Delta>"
     by (rule reds_doesnt_forget[OF distinct_redsD1[OF Variable.hyps(2)]])
 
-  have new_fresh: "(heapVars \<Delta> - (heapVars \<Gamma> - {x})) \<inter> fdom \<rho> = {}"
-    using reds_avoids_live[OF distinct_redsD1[OF Variable.hyps(2)]] 2
+  have "fv (delete x \<Gamma>, e) \<union> {x} = fv (\<Gamma>, Var x)"
+    by (rule fv_delete_heap[OF `distinctVars \<Gamma>` `(x,e)\<in>set \<Gamma>`])
+  hence prem: "fv (delete x \<Gamma>, e) - heapVars (delete x \<Gamma>) \<subseteq> set (x # L)" using 2 by auto
+
+  have fv_subset: "fv (delete x \<Gamma>, e) - heapVars (delete x \<Gamma>) \<subseteq> - (heapVars \<Delta> - heapVars \<Gamma>)"
+    apply (rule subset_trans[OF prem])
+    apply (rule subset_trans[OF reds_avoids_live'[OF distinct_redsD1[OF Variable.hyps(2)]]])
     by auto
 
-  have [simp]: "insert x (fdom \<rho> \<union> (heapVars \<Gamma> - {x})) - heapVars \<Delta> = insert x (fdom \<rho> - heapVars \<Gamma>)"
-    using new_fresh subset `x \<notin> _` by auto
-
-  have [simp]: "insert x (fdom \<rho> \<union> heapVars \<Delta>) - heapVars \<Delta> = insert x (fdom \<rho> - heapVars \<Gamma>)"
-    using new_fresh subset `x \<notin> _` by auto
-
-  have [simp]: "(insert x (fdom \<rho> \<union> (heapVars \<Gamma> - {x})) \<inter> heapVars \<Delta>) = heapVars \<Gamma> - {x}"
-    using new_fresh subset `x \<notin> _` by auto
-
-  have [simp]:"\<And> x y . x \<union> y \<union> y = x \<union> y" "\<And> x y. (x \<union> y) \<inter> y = y"
-    by auto
-
-  have [simp]: "insert x (fdom \<rho> \<union> (heapVars \<Gamma> - {x})) - (heapVars  \<Gamma> - {x}) = insert x (fdom \<rho> - heapVars \<Gamma>)"
-    by auto
-
-  have [simp]: "(heapVars \<Gamma> - {x}) \<inter> (fdom \<rho> \<union> (heapVars \<Gamma> - {x})) = (heapVars \<Gamma> - {x})"
-    by auto
-
-  have [simp]: "(fdom \<rho> - heapVars \<Gamma>) \<inter> (fdom \<rho> \<union> (heapVars \<Gamma> - {x})) = (fdom \<rho> - heapVars \<Gamma>)"
-    by auto
-
+  let "?new" = "heapVars \<Delta> - heapVars \<Gamma>"
+  have "heapVars \<Gamma> \<subseteq> (-?new)" by auto
 
   have "\<N>\<lbrace>\<Gamma>\<rbrace>\<rho> = \<N>\<lbrace>(x,e) # delete x \<Gamma>\<rbrace>\<rho>"
-    apply (rule HSem_reorder)
-    apply (rule distinctVars_map_of_delete_insert[symmetric, OF Variable(5,1)])
-    done
-    thm iterative_HSem
+    by (rule HSem_reorder[OF distinctVars_map_of_delete_insert[symmetric, OF Variable(5,1)]])
   also have "\<dots> = (\<mu> \<rho>'. (\<rho> f++\<^bsub>(heapVars (delete x \<Gamma>))\<^esub> (\<N>\<lbrace>delete x \<Gamma>\<rbrace>\<rho>'))( x f\<mapsto> \<N>\<lbrakk> e \<rbrakk>\<^bsub>\<rho>'\<^esub>))"
     by (rule iterative_HSem, simp)
   also have "\<dots> = (\<mu> \<rho>'. (\<rho> f++\<^bsub>(heapVars (delete x \<Gamma>))\<^esub> (\<N>\<lbrace>delete x \<Gamma>\<rbrace>\<rho>'))( x f\<mapsto> \<N>\<lbrakk> e \<rbrakk>\<^bsub>\<N>\<lbrace>delete x \<Gamma>\<rbrace>\<rho>'\<^esub>))"
     by (rule iterative_HSem', simp)
   finally
-  have "\<N>\<lbrace>\<Gamma>\<rbrace>\<rho> \<sqsubseteq>  ..." by (rule ssubst) (rule below_refl)
-  also have "\<dots> \<sqsubseteq> (\<mu> \<rho>'. (\<rho> f++\<^bsub>heapVars \<Delta>\<^esub> (\<N>\<lbrace>\<Delta>\<rbrace>\<rho>'))( x f\<mapsto> \<N>\<lbrakk> z \<rbrakk>\<^bsub>\<N>\<lbrace>\<Delta>\<rbrace>\<rho>'\<^esub>))"
-    apply (rule parallel_fix_ind)
-    apply (intro adm_is_adm_on adm_lemmas lookup_cont  cont2cont_lambda cont2cont)
-    apply simp
-    apply (rule fmap_belowI)
-    apply (case_tac "xaa = x")
-    sorry
-    (*
-    apply simp
-    apply (rule below_trans[OF Variable.hyps(3)])
-    using 2 apply auto[1]
-    apply (erule ESem_mono_relaxed[OF HSem_monofun_relaxed])
-
-    apply (case_tac "xa \<in> heapVars \<Gamma>")
-    apply (subgoal_tac "xa \<in> heapVars \<Delta>")
-      prefer 2
-      using subset apply auto[1]
-    apply simp
-    using Variable.hyps(4)
-    apply (erule_tac x = "y" in meta_allE)
-    apply (elim meta_impE)
-    using 2  `x \<notin> heapVars \<Delta>` apply auto[1]
-    apply (drule_tac  x = xa in fun_belowD) back
-    apply simp
-    apply (erule below_trans)
-    apply (drule HSem_monofun_relaxed)
-    apply (drule_tac  x = xa in fun_belowD)
-    apply simp
-
-    apply (case_tac "xa \<in> fdom \<rho>")
-    apply (subgoal_tac "xa \<notin> heapVars \<Delta>")
-      prefer 2
-      using new_fresh apply auto[1]
-    apply simp
-    apply simp
-    done
-    *)
-  also have "\<dots> = (\<mu> \<rho>'. (\<rho> f++\<^bsub>heapVars \<Delta>\<^esub> (\<N>\<lbrace>\<Delta>\<rbrace>\<rho>'))( x f\<mapsto> \<N>\<lbrakk> z \<rbrakk>\<^bsub>\<rho>'\<^esub>))"
+  have "(\<N>\<lbrace>\<Gamma>\<rbrace>\<rho>)f|` (- ?new) \<sqsubseteq> (...) f|` (- ?new)" by (rule ssubst) (rule below_refl)
+  also have "\<dots> \<sqsubseteq> (\<mu> \<rho>'. (\<rho> f++\<^bsub>heapVars \<Delta>\<^esub> (\<N>\<lbrace>\<Delta>\<rbrace>\<rho>'))( x f\<mapsto> \<N>\<lbrakk> z \<rbrakk>\<^bsub>\<N>\<lbrace>\<Delta>\<rbrace>\<rho>'\<^esub>)) f|` (- ?new)"
+  proof (induction rule: parallel_fix_ind)
+    case 1 show ?case by simp
+  next
+    case 2 show ?case ..
+  next
+    case (3 \<sigma> \<sigma>')
+    hence "\<N>\<lbrakk> e \<rbrakk>\<^bsub>\<N>\<lbrace>delete x \<Gamma>\<rbrace>\<sigma>\<^esub> \<sqsubseteq> \<N>\<lbrakk> e \<rbrakk>\<^bsub>\<N>\<lbrace>delete x \<Gamma>\<rbrace>\<sigma>'\<^esub>"
+      and "(\<N>\<lbrace>delete x \<Gamma>\<rbrace>\<sigma>) f|` heapVars (delete x \<Gamma>) \<sqsubseteq> (\<N>\<lbrace>delete x \<Gamma>\<rbrace>\<sigma>') f|` heapVars (delete x \<Gamma>)"
+      using fv_subset by (auto intro: ESem_fresh_cong_below HSem_fresh_cong_below  fmap_restr_below_subset[OF _ 3])
+    from below_trans[OF this(1) Variable(3)[OF prem]] below_trans[OF this(2) Variable(4)[OF prem]]
+    have  "\<N>\<lbrakk> e \<rbrakk>\<^bsub>\<N>\<lbrace>delete x \<Gamma>\<rbrace>\<sigma>\<^esub> \<sqsubseteq> \<N>\<lbrakk> z \<rbrakk>\<^bsub>\<N>\<lbrace>\<Delta>\<rbrace>\<sigma>'\<^esub>"
+       and "(\<N>\<lbrace>delete x \<Gamma>\<rbrace>\<sigma>) f|` heapVars (delete x \<Gamma>) \<sqsubseteq> (\<N>\<lbrace>\<Delta>\<rbrace>\<sigma>') f|` heapVars (delete x \<Gamma>)".
+    thus ?case
+      using subset
+      by (auto intro!: fmap_belowI simp add: lookup_fmap_add_eq lookup_fmap_upd_eq lookup_fmap_restr_eq elim: fmap_restr_belowD)
+  qed
+  also have "\<dots> = (\<mu> \<rho>'. (\<rho> f++\<^bsub>heapVars \<Delta>\<^esub> (\<N>\<lbrace>\<Delta>\<rbrace>\<rho>'))( x f\<mapsto> \<N>\<lbrakk> z \<rbrakk>\<^bsub>\<rho>'\<^esub>)) f|` (-?new)"
     by (rule arg_cong[OF iterative_HSem'[symmetric], OF `x \<notin> heapVars \<Delta>`])
-  also have "\<dots> = \<N>\<lbrace>(x,z) # \<Delta>\<rbrace>\<rho>"
+  also have "\<dots> = (\<N>\<lbrace>(x,z) # \<Delta>\<rbrace>\<rho>)  f|` (-?new)"
     by (rule arg_cong[OF iterative_HSem[symmetric], OF `x \<notin> heapVars \<Delta>`])
   finally
-  show le: ?case.
+  show le: ?case by (rule fmap_restr_below_subset[OF `heapVars \<Gamma> \<subseteq> (-?new)`])
 
   have "\<N>\<lbrakk> Var x \<rbrakk>\<^bsub>\<N>\<lbrace>\<Gamma>\<rbrace>\<rho>\<^esub> \<sqsubseteq> \<N>\<lbrakk> Var x \<rbrakk>\<^bsub>\<N>\<lbrace>(x, z) # \<Delta>\<rbrace>\<rho>\<^esub>"
     apply (rule cfun_belowI)
@@ -176,24 +162,18 @@ case (Let as \<Gamma> L body \<Delta> z)
   case 1
   { fix a
     assume a: "a \<in> heapVars (asToHeap as)"
-    have "atom a \<sharp> L" 
-      by (rule Let(2)[unfolded fresh_star_def set_bn_to_atom_heapVars, rule_format, OF imageI[OF a]])
-    hence "a \<notin> set L"
-      by (metis fresh_list_elem not_self_fresh)
-    moreover
     have "atom a \<sharp> \<Gamma>" 
       by (rule Let(1)[unfolded fresh_star_def set_bn_to_atom_heapVars, rule_format, OF imageI[OF a]])
     hence "a \<notin> heapVars \<Gamma>"
       by (metis heapVars_not_fresh)
-    ultimately
-    have "a \<notin> fdom \<rho>" and "a \<notin> heapVars \<Gamma>"
-      using 1 by auto
   }
   note * = this
-  
-  have hyp: "fdom \<rho> - heapVars (asToHeap as @ \<Gamma>) \<subseteq> set L"
-    using 1 by auto
 
+  
+  have "fv (asToHeap as @ \<Gamma>, body) - heapVars (asToHeap as @ \<Gamma>) \<subseteq>  fv (\<Gamma>, Let as body) - heapVars \<Gamma>"
+    by (auto dest: set_mp[OF fv_asToHeap])
+  with 1 have prem: "fv (asToHeap as @ \<Gamma>, body) - heapVars (asToHeap as @ \<Gamma>) \<subseteq> set L" by auto
+  
   have f1: "atom ` heapVars (asToHeap as) \<sharp>* \<Gamma>"
     using Let(1) by (simp add: set_bn_to_atom_heapVars)
 
@@ -205,21 +185,40 @@ case (Let as \<Gamma> L body \<Delta> z)
   also have "\<dots> =  \<N>\<lbrakk> body \<rbrakk>\<^bsub>\<N>\<lbrace>asToHeap as @ \<Gamma>\<rbrace>\<rho>\<^esub>"
     by (rule arg_cong[OF HSem_merge[OF f1]])
   also have "\<dots> \<sqsubseteq>  \<N>\<lbrakk> z \<rbrakk>\<^bsub>\<N>\<lbrace>\<Delta>\<rbrace>\<rho>\<^esub>"
-    by (rule Let.hyps(4)[OF hyp])
+    by (rule Let.hyps(4)[OF prem])
   finally
   show ?case.
 
-  have "\<N>\<lbrace>\<Gamma>\<rbrace>\<rho> \<sqsubseteq> \<N>\<lbrace>asToHeap as\<rbrace>(\<N>\<lbrace>\<Gamma>\<rbrace>\<rho>)"
+  have "(\<N>\<lbrace>\<Gamma>\<rbrace>\<rho>) f|` (heapVars \<Gamma>) \<sqsubseteq> (\<N>\<lbrace>asToHeap as\<rbrace>(\<N>\<lbrace>\<Gamma>\<rbrace>\<rho>)) f|` (heapVars \<Gamma>)"
     apply (rule fmap_belowI)
     apply (case_tac "x \<in> heapVars (asToHeap as)")
-    apply (auto simp add: the_lookup_HSem_heap the_lookup_HSem_other * )
-    (* done *)
-    sorry
-  also have "\<dots> = \<N>\<lbrace>asToHeap as @ \<Gamma>\<rbrace>\<rho>"
+    apply (auto simp add: the_lookup_HSem_other lookup_fmap_restr_eq *)
+    done
+  also have "\<dots> = (\<N>\<lbrace>asToHeap as @ \<Gamma>\<rbrace>\<rho>) f|` (heapVars \<Gamma>)"
     by (rule arg_cong[OF HSem_merge[OF f1]])
-  also have "\<dots> \<sqsubseteq> \<N>\<lbrace>\<Delta>\<rbrace>\<rho>"
-    by (rule Let.hyps(5)[OF hyp])
+  also have "\<dots> \<sqsubseteq> (\<N>\<lbrace>\<Delta>\<rbrace>\<rho>) f|` (heapVars \<Gamma>)"
+    by (rule fmap_restr_below_subset[OF _ Let.hyps(5)[OF prem]]) simp
   finally
-  show "\<N>\<lbrace>\<Gamma>\<rbrace>\<rho> \<sqsubseteq> \<N>\<lbrace>\<Delta>\<rbrace>\<rho>".
+  show "(\<N>\<lbrace>\<Gamma>\<rbrace>\<rho>) f|` heapVars \<Gamma> \<sqsubseteq> (\<N>\<lbrace>\<Delta>\<rbrace>\<rho>) f|` heapVars \<Gamma>".
 qed
+
+
+corollary correctness_empty_env:
+  assumes "\<Gamma> : e \<Down>\<^bsub>L\<^esub> \<Delta> : z"
+  and     "distinctVars \<Gamma>"
+  and     "fv (\<Gamma>, e) \<subseteq> set L"
+  shows   "\<N>\<lbrakk>e\<rbrakk>\<^bsub>\<N>\<lbrace>\<Gamma>\<rbrace>\<^esub> \<sqsubseteq> \<N>\<lbrakk>z\<rbrakk>\<^bsub>\<N>\<lbrace>\<Delta>\<rbrace>\<^esub>" and "\<N>\<lbrace>\<Gamma>\<rbrace> \<sqsubseteq> \<N>\<lbrace>\<Delta>\<rbrace>"
+proof-
+  from assms(3) have "fv (\<Gamma>, e) - heapVars \<Gamma> \<subseteq> set L" by auto
+  note corr =  correctness[OF assms(1,2) this, where \<rho> = "f\<emptyset>"]
+
+  show "\<N>\<lbrakk> e \<rbrakk>\<^bsub>\<N>\<lbrace>\<Gamma>\<rbrace>\<^esub> \<sqsubseteq> \<N>\<lbrakk> z \<rbrakk>\<^bsub>\<N>\<lbrace>\<Delta>\<rbrace>\<^esub>" using corr(1).
+
+  have "\<N>\<lbrace>\<Gamma>\<rbrace> = (\<N>\<lbrace>\<Gamma>\<rbrace>) f|` heapVars \<Gamma> "
+    using fmap_restr_useless[OF HSem_fdom_subset, where \<rho>1 = "f\<emptyset>"] by simp
+  also have "\<dots> \<sqsubseteq> (\<N>\<lbrace>\<Delta>\<rbrace>) f|` heapVars \<Gamma>" using corr(2).
+  also have "\<dots> \<sqsubseteq> \<N>\<lbrace>\<Delta>\<rbrace>" by (rule fmap_restr_below_itself)
+  finally show "\<N>\<lbrace>\<Gamma>\<rbrace> \<sqsubseteq> \<N>\<lbrace>\<Delta>\<rbrace>".
+qed
+
 end
