Launchbury/Nominal-Utils.thy
@@ -193,10 +193,14 @@ definition fv :: "'a::pt \<Rightarrow> 'b::at_base set" where "fv e = {v. atom v
 lemma fv_eqvt[simp,eqvt]: "\<pi> \<bullet> (fv e) = fv (\<pi> \<bullet> e)"
   unfolding fv_def by simp
 
+lemma fv_Nil[simp]: "fv [] = {}"
+  by (auto simp add: fv_def supp_Nil)
 lemma fv_Cons[simp]: "fv (x # xs) = fv x \<union> fv xs"
   by (auto simp add: fv_def supp_Cons)
 lemma fv_Pair[simp]: "fv (x, y) = fv x \<union> fv y"
   by (auto simp add: fv_def supp_Pair)
+lemma fv_append[simp]: "fv (x @ y) = fv x \<union> fv y"
+  by (auto simp add: fv_def supp_append)
 lemma fv_at_base[simp]: "fv a = {a::'a::at_base}"
   by (auto simp add: fv_def supp_at_base)
 
